cpdt/src/CpdtTactics.v
@@ -32,18 +32,35 @@ Definition inject {A} (x : A) : tactic :=
   try subst.
 
 (** Try calling tactic function [f] on all hypotheses, keeping the first application that doesn't fail. *)
-Ltac appHyps f :=
-  match goal with
-    | [ H : _ |- _ ] => f H
+Definition appHyps {A B} (f : A -> gtactic B) : gtactic B :=
+  match_goal with
+  | [[ H : A |- B ]] => f H
   end.
 
 (** Succeed iff [x] is in the list [ls], represented with left-associated nested tuples. *)
-Ltac inList x ls :=
-  match ls with
+Ltac linList x ls :=
+  lazymatch ls with
     | x => idtac
     | (_, x) => idtac
-    | (?LS, _) => inList x LS
+    | (?LS, _) => linList x LS
   end.
+
+Fixpoint inList {A} (x : A) (ls : mlist A) : tactic :=
+    match ls with (** check that mtac unification is the same as ltac here... *)
+    | [m:]    => fun _ => M.failwith "omg"
+    | y :m: ls' => mmatch y with
+            | x => idtac
+            | _ => inList x ls'
+    end
+end%mlist.
+
+Ltac tuple_to_list ls :=
+  match ls with
+  | (?LS, ?X) => let r := tuple_to_list LS in constr:(Dyn X :m: r)
+  | ?X => constr:([m: Dyn X])
+  end.
+
+Check ltac:(let o := tuple_to_list (1,2,3,4) in pose o).
 
 (** Try calling tactic function [f] on every element of tupled list [ls], keeping the first call not to fail. *)
 Ltac app f ls :=
@@ -65,8 +82,82 @@ Ltac all f ls :=
 Ltac simplHyp invOne :=
   (** Helper function to do inversion on certain hypotheses, where [H] is the hypothesis and [F] its head symbol *)
   let invert H F :=
+    idtac "start-simpl";
+    idtac invOne;
+    idtac F;
+    match goal with
+    | |- ?g => idtac g
+    end;
     (** We only proceed for those predicates in [invOne]. *)
-    inList F invOne;
+    linList F invOne;
+    idtac "in-list";
+    (*mrun (inList (Dyn F) ltac:(tuple_to_list invOne));*)
+    (** This case covers an inversion that succeeds immediately, meaning no constructors of [F] applied. *)
+      (inversion H; fail)
+    (** Otherwise, we only proceed if inversion eliminates all but one constructor case. *)
+      || (inversion H; [idtac]; clear H; try subst) in
+
+  match goal with
+    (** Eliminate all existential hypotheses. *)
+    | [ H : ex _ |- _ ] => destruct H
+
+    (** Find opportunities to take advantage of injectivity of data constructors, for several different arities. *)
+    | [ H : ?F ?X = ?F ?Y |- ?G ] =>
+      (** This first branch of the [||] fails the whole attempt iff the arguments of the constructor applications are already easy to prove equal. *)
+      (assert (X = Y); [ assumption | fail 1 ])
+      (** If we pass that filter, then we use injection on [H] and do some simplification as in [inject].
+         * The odd-looking check of the goal form is to avoid cases where [injection] gives a more complex result because of dependent typing, which we aren't equipped to handle here. *)
+      || (injection H;
+        match goal with
+          | [ |- X = Y -> G ] =>
+            try clear H; intros; try subst
+        end)
+    | [ H : ?F ?X ?U = ?F ?Y ?V |- ?G ] =>
+      (assert (X = Y); [ assumption
+        | assert (U = V); [ assumption | fail 1 ] ])
+      || (injection H;
+        match goal with
+          | [ |- U = V -> X = Y -> G ] =>
+            try clear H; intros; try subst
+        end)
+
+    (** Consider some different arities of a predicate [F] in a hypothesis that we might want to invert. *)
+    | [ H : ?F _ |- _ ] => invert H F
+    | [ H : ?F _ _ |- _ ] => invert H F
+    | [ H : ?F _ _ _ |- _ ] => invert H F
+    | [ H : ?F _ _ _ _ |- _ ] => invert H F
+    | [ H : ?F _ _ _ _ _ |- _ ] => invert H F
+
+    (** Use an (axiom-dependent!) inversion principle for dependent pairs, from the standard library. *)
+    | [ H : existT _ ?T _ = existT _ ?T _ |- _ ] => generalize (inj_pair2 _ _ _ _ _ H); clear H
+
+    (** If we're not ready to use that principle yet, try the standard inversion, which often enables the previous rule. *)
+    | [ H : existT _ _ _ = existT _ _ _ |- _ ] => inversion H; clear H
+
+    (** Similar logic to the cases for constructor injectivity above, but specialized to [Some], since the above cases won't deal with polymorphic constructors. *)
+    | [ H : Some _ = Some _ |- _ ] => injection H; clear H
+  end.
+
+(** Workhorse tactic to simplify hypotheses for a variety of proofs.
+   * Argument [invOne] is a tuple-list of predicates for which we always do inversion automatically. *)
+Ltac simplHyp' invOne :=
+  (** Helper function to do inversion on certain hypotheses, where [H] is the hypothesis and [F] its head symbol *)
+  let invert H F :=
+    idtac "start-simpl";
+    let omg := tuple_to_list invOne in
+    idtac omg;
+    idtac F;
+    match goal with
+    | |- ?g => idtac g
+    end;
+    (** We only proceed for those predicates in [invOne]. *)
+    (*linList F invOne;*)
+    let omg' := mrun (inList (Dyn F) ltac:(tuple_to_list invOne)) in
+    idtac "help me" omg';
+    let list := tuple_to_list invOne in
+    mrun (inList (Dyn F) list);
+    idtac "in-list";
+
     (** This case covers an inversion that succeeds immediately, meaning no constructors of [F] applied. *)
       (inversion H; fail)
     (** Otherwise, we only proceed if inversion eliminates all but one constructor case. *)
@@ -185,19 +276,55 @@ Require Import JMeq.
    * - A tuple-list of lemmas we try [inster]-ing
    * - A tuple-list of predicates we try inversion for *)
 Ltac crush' lemmas invOne :=
+  idtac lemmas;
   (** A useful combination of standard automation *)
-  let sintuition := simpl in *; intuition; try subst;
-    repeat (simplHyp invOne; intuition; try subst); try congruence in
+  let sintuition := idtac "start-int"; simpl in *; intuition; try subst;
+    repeat (simplHyp invOne; intuition; try subst); try congruence; idtac "end-int" in
 
   (** A fancier version of [rewriter] from above, which uses [crush'] to discharge side conditions *)
-  let rewriter := autorewrite with core in *;
+  let rewriter := idtac "start-rew"; autorewrite with core in *;
     repeat (match goal with
               | [ H : ?P |- _ ] =>
                 match P with
                   | context[JMeq] => fail 1 (** JMeq is too fancy to deal with here. *)
                   | _ => rewrite H by crush' lemmas invOne
                 end
-            end; autorewrite with core in *) in
+            end; autorewrite with core in *); idtac "end-rew" in
+
+  (** Now the main sequence of heuristics: *)
+    (sintuition; idtac "omg"; rewriter;
+      match lemmas with
+        | false => idtac (** No lemmas?  Nothing to do here *)
+        | _ =>
+          (** Try a loop of instantiating lemmas... *)
+          repeat ((app ltac:(fun L => inster L L) lemmas
+          (** ...or instantiating hypotheses... *)
+            || mrun (appHyps ltac:(fun L => inster L L)));
+          (** ...and then simplifying hypotheses. *)
+          repeat (simplHyp invOne; intuition)); un_done
+      end;
+      idtac "omg-2"; sintuition; idtac "omg-3"; rewriter; idtac "omg-4"; sintuition;
+      (** End with a last attempt to prove an arithmetic fact with [omega], or prove any sort of fact in a context that is contradictory by reasoning that [omega] can do. *)
+      try omega; try (elimtype False; omega)).
+
+
+(** A more parameterized version of the famous [crush].  Extra arguments are:
+   * - A tuple-list of lemmas we try [inster]-ing
+   * - A tuple-list of predicates we try inversion for *)
+Ltac crush'' lemmas invOne :=
+  (** A useful combination of standard automation *)
+  let sintuition := idtac "start-int"; simpl in *; intuition; try subst;
+    repeat (simplHyp' invOne; intuition; try subst); try congruence; idtac "end-int" in
+
+  (** A fancier version of [rewriter] from above, which uses [crush'] to discharge side conditions *)
+  let rewriter := idtac "start-rew"; autorewrite with core in *;
+    repeat (match goal with
+              | [ H : ?P |- _ ] =>
+                match P with
+                  | context[JMeq] => fail 1 (** JMeq is too fancy to deal with here. *)
+                  | _ => rewrite H by crush'' lemmas invOne
+                end
+            end; autorewrite with core in *); idtac "end-rew" in
 
   (** Now the main sequence of heuristics: *)
     (sintuition; rewriter;
@@ -207,11 +334,11 @@ Ltac crush' lemmas invOne :=
           (** Try a loop of instantiating lemmas... *)
           repeat ((app ltac:(fun L => inster L L) lemmas
           (** ...or instantiating hypotheses... *)
-            || appHyps ltac:(fun L => inster L L));
+            || mrun (appHyps ltac:(fun L => inster L L)));
           (** ...and then simplifying hypotheses. *)
-          repeat (simplHyp invOne; intuition)); un_done
+          repeat (simplHyp' invOne; intuition)); un_done
       end;
-      sintuition; rewriter; sintuition;
+      sintuition; idtac "omg-2"; rewriter; idtac "omg-3"; sintuition;
       (** End with a last attempt to prove an arithmetic fact with [omega], or prove any sort of fact in a context that is contradictory by reasoning that [omega] can do. *)
       try omega; try (elimtype False; omega)).
 
